Improve dont_lift in clos_op and remove a cheat

compiler/backend/clos_opScript.sml
@@ -26,17 +26,22 @@ Proof
 QED
 
 Definition dest_Build_def:
-  dest_Build (Build [i]) = SOME i ∧
+  dest_Build (Build [Str s]) = SOME (Str s) ∧
+  dest_Build (Build [W64 w]) = SOME (W64 w) ∧
   dest_Build _ = NONE
 End
 
 Theorem dest_Build_pmatch:
-  dest_Build x = case x of Build [i] => SOME i | _ => NONE
+  dest_Build x = case x of
+                 | Build [Str s] => SOME (Str s)
+                 | Build [W64 w] => SOME (W64 w)
+                 | _ => NONE
 Proof
   CONV_TAC(RAND_CONV patternMatchesLib.PMATCH_ELIM_CONV)
   \\ Cases_on ‘x’ \\ EVAL_TAC
   \\ Cases_on ‘l’ \\ fs [dest_Build_def]
   \\ Cases_on ‘t’ \\ fs [dest_Build_def]
+  \\ Cases_on ‘h’ \\ fs [dest_Build_def]
 QED
 
 Definition dest_Cons_def:
@@ -332,7 +337,10 @@ Definition dont_lift_def:
     | NONE =>
       dtcase dest_Op_Cons_Nil x of
       | SOME t => T
-      | NONE => F
+      | NONE =>
+        dtcase dest_Op_Build x of
+        | SOME t => T
+        | NONE => F
 End
 
 Definition lift_exps_def:
