compiler/backend/proofs/clos_opProofScript.sml
@@ -45,11 +45,14 @@ Proof
 QED
 
 Theorem dest_Build_thm:
-  dest_Build x = SOME i ⇔ x = Build [i]
+  dest_Build x = SOME i ⇔
+  ∃s w. x = Build [i] ∧ (i = Str s ∨ i = W64 w)
 Proof
   Cases_on ‘x’ \\ fs [dest_Build_def]
   \\ Cases_on ‘l’ \\ fs [dest_Build_def]
   \\ Cases_on ‘t’ \\ fs [dest_Build_def]
+  \\ Cases_on ‘h’ \\ fs [dest_Build_def]
+  \\ Cases_on ‘i’ \\ fs []
 QED
 
 Theorem dest_Cons_thm:
@@ -86,22 +89,19 @@ Proof
   THEN1
    (gvs [eq_direct_build_def,AllCaseEqs(),dest_Op_Nil_thm,dest_Build_thm]
     \\ fs [evaluate_def,do_app_def]
-    THEN1
+    \\ TRY
      (Cases_on ‘evaluate ([x],env,s)’ \\ fs [] \\ Cases_on ‘q’ \\ fs []
-      \\ Cases_on ‘p’ \\ fs []
       \\ rw [] \\ fs [evaluate_def]
       \\ imp_res_tac evaluate_SING \\ gvs []
-      \\ Cases_on ‘r1’ \\ gvs [do_eq_def,do_app_def] \\ eq_tac \\ rw[])
-    THEN1
+      \\ Cases_on ‘r1’ \\ gvs [do_eq_def,do_app_def] \\ eq_tac \\ rw[] \\ NO_TAC)
+    \\ TRY
      (Cases_on ‘evaluate ([y],env,s)’ \\ fs [] \\ Cases_on ‘q’ \\ fs []
-      \\ Cases_on ‘p’ \\ fs []
       \\ rw [] \\ fs [evaluate_def]
       \\ imp_res_tac evaluate_SING \\ gvs []
-      \\ Cases_on ‘r1’ \\ gvs [do_eq_def,do_app_def]
-      \\ rw [] \\ eq_tac \\ rw [])
-    \\ Cases_on ‘p’ \\ Cases_on ‘q’ \\ gvs []
-    \\ EVAL_TAC \\ rw [] \\ fs [] \\ EVAL_TAC
-    \\ gvs [GSYM mlstringTheory.explode_def]
+      \\ Cases_on ‘r1’ \\ gvs [do_eq_def,do_app_def] \\ eq_tac \\ rw[] \\ NO_TAC)
+    \\ fs [do_eq_def] \\ rw [evaluate_MakeBool]
+    \\ fs [do_eq_def] \\ rw [evaluate_MakeBool]
+    \\ eq_tac \\ rw [] \\ CCONTR_TAC
     \\ rename [‘ss ≠ tt’]
     \\ Cases_on ‘ss’ \\ Cases_on ‘tt’ \\ fs []
     \\ pop_assum mp_tac
@@ -131,11 +131,18 @@ QED
 Theorem dont_lift_thm:
   dont_lift x ⇔
   (∃t n. x = Op t (Cons n) []) ∨
-  (∃t i. x = Op t (Const i) [])
+  (∃t i. x = Op t (Const i) []) ∨
+  (∃t s. x = Op t (Build [Str s]) []) ∨
+  (∃t w. x = Op t (Build [W64 w]) [])
 Proof
   Cases_on ‘x’ \\ fs [dont_lift_def,dest_Op_Nil_def,dest_Op_def]
   \\ Cases_on ‘o'’ \\ fs [dest_Const_def,dest_Cons_def]
-  \\ Cases_on ‘l’ \\ fs [dest_Const_def,dest_Cons_def]
+  \\ Cases_on ‘l’ \\ fs [dest_Const_def,dest_Cons_def,dest_Build_def]
+  \\ rename [‘Build ll’]
+  \\ Cases_on ‘ll’ \\ fs [dest_Const_def,dest_Cons_def,dest_Build_def]
+  \\ rename [‘Build (hh::ll)’]
+  \\ Cases_on ‘ll’ \\ fs [dest_Const_def,dest_Cons_def,dest_Build_def]
+  \\ Cases_on ‘hh’ \\ fs [dest_Const_def,dest_Cons_def,dest_Build_def]
 QED
 
 Theorem dont_lift_pure:
@@ -306,8 +313,12 @@ Inductive simple_exp:
   (∀t i. simple_exp (Var t i)) ∧
   (∀t x y z. simple_exp x ∧ simple_exp y ∧ simple_exp z ⇒ simple_exp (If t x y z)) ∧
   (∀t i. simple_exp (Op t (Const i) [])) ∧
+  (∀t i. simple_exp (Op t (Build [Str i]) [])) ∧
+  (∀t i. simple_exp (Op t (Build [W64 i]) [])) ∧
   (∀t i xs. EVERY simple_exp xs ⇒ simple_exp (Op t (Cons i) xs)) ∧
-  (∀t i x. simple_exp x ⇒ simple_exp (Op t (EqualConst i) [x])) ∧
+  (∀t i x. simple_exp x ⇒ simple_exp (Op t (EqualConst (Int i)) [x])) ∧
+  (∀t i x. simple_exp x ⇒ simple_exp (Op t (EqualConst (Str i)) [x])) ∧
+  (∀t i x. simple_exp x ⇒ simple_exp (Op t (EqualConst (W64 i)) [x])) ∧
   (∀t i x. simple_exp x ⇒ simple_exp (Op t (ElemAt i) [x])) ∧
   (∀t x y. simple_exp x ∧ simple_exp y ⇒ simple_exp (Op t Equal [x;y])) ∧
   (∀t l y x. simple_exp x ⇒ simple_exp (Op t (TagLenEq l y) [x]))
@@ -392,6 +403,7 @@ Theorem eq_direct_simple_exp:
 Proof
   fs [eq_direct_def,AllCaseEqs(),eq_direct_const_def,eq_direct_nil_def,eq_direct_build_def]
   \\ rw [MakeBool_def] \\ simp [Once simple_exp_cases]
+  \\ gvs [dest_Op_Nil_thm,dest_Build_thm]
 QED
 
 Theorem simple_exp_eq_pure_list:
@@ -685,11 +697,12 @@ QED
 
 Inductive red_rel:
 [red_rel_Op:]
-  (∀xs ys t op i tag t1 t2 p ps.
+  (∀xs ys t op i tag t1 t2 s w.
     red_rel xs ys ∧
     MEM op [Add;Sub;Mult;Div;Mod;Less;LessEq;Greater;GreaterEq;Equal;Const i;
-            Cons tag; TagEq tag; TagLenEq t1 t2; LenEq n; EqualConst p;
-            ElemAt t1; Build ps] ⇒
+            Cons tag; TagEq tag; TagLenEq t1 t2; LenEq n;
+            EqualConst (Str s); EqualConst (W64 w); EqualConst (Int i);
+            ElemAt t1; Build [Str s]; Build [W64 w]] ⇒
     red_rel [Op t op xs] ys)
   ∧
   (red_rel [] [])
@@ -817,8 +830,10 @@ Proof
     \\ gvs [dont_lift_def,AllCaseEqs()]
     \\ Cases_on ‘dest_Op_Nil dest_Const x’ \\ gvs [dest_Op_Nil_thm]
     \\ Cases_on ‘dest_Op_Nil dest_Cons x’ \\ gvs [dest_Op_Nil_thm]
+    \\ Cases_on ‘dest_Op_Nil dest_Build x’ \\ gvs [dest_Op_Nil_thm]
     \\ gvs [dest_Cons_thm]
     \\ gvs [dest_Const_thm]
+    \\ gvs [dest_Build_thm]
     \\ simp [Once red_rel_cases]
     \\ simp [Once red_rel_cases])
   \\ Cases_on ‘dest_Op dest_Cons x’ \\ gvs []
@@ -853,11 +868,11 @@ Proof
   \\ gvs [eq_direct_nil_def,AllCaseEqs(),MakeBool_def]
   \\ irule_at Any red_rel_Op \\ fs []
   \\ gvs [dest_Op_Nil_thm,dest_Cons_thm,dest_Const_thm,dest_Build_thm]
-  \\ irule_at Any red_rel_multi \\ fs []
+  \\ TRY (irule_at Any red_rel_multi \\ fs []
   \\ rpt (irule_at Any red_rel_Op \\ fs [])
   \\ fs [red_rel_nil]
   \\ simp [Once red_rel_cases]
-  \\ metis_tac []
+  \\ metis_tac [])
 QED
 
 Theorem red_rel_refl:
@@ -1016,7 +1031,6 @@ Proof
   \\ ho_match_mp_tac red_rel_ind
   \\ fs [no_Labels_def]
   \\ rw [] \\ fs [] \\ eq_tac \\ rw []
-  \\ cheat (* hmm *)
 QED
 
 Theorem obeys_max_app_SmartOp:
